Approximate implementation of checker function. Next steps registered on Nov.23 page

curry.v
@@ -4,53 +4,127 @@ Import M.notations.
 Import M.M.
 
 Local Notation MFA T := (MTele_val (MTele_C SType SProp M T)).
+Local Notation InF s n := (forall now_ty : forall s0 : Sort, MTele_Sort s0 n -> s0, (forall (s0 : Sort) (T : MTele_Sort s0 n), MTele_val T -> now_ty s0 T) -> s).
 
 (* If recursion is needed then it's TyTree, if not only Type *)
 Inductive TyTree : Type :=
-| tyTree_M (p : bool) (T : Type) : TyTree
-| tyTree_imp (p : bool) (T R : TyTree) : TyTree
-| tyTree_FATele (P : bool) {m : MTele} (T : MTele_Ty m) (F : forall t : MTele_val T, TyTree) : TyTree  
-| tyTree_FA (p : bool) (T : Type) (F : T -> TyTree) : TyTree
-| tyTree_FAType (p : bool) (F : Type -> Type) : TyTree
-| tyTree_ow (p : bool) (T : Type) : TyTree
+| tyTree_val {m : MTele} (T : MTele_Ty m) : TyTree
+| tyTree_M (T : Type) : TyTree
+| tyTree_MFA {m : MTele} (T : MTele_Ty m) : TyTree
+| tyTree_In (s : Sort) {m : MTele} (F : InF s m) : TyTree
+| tyTree_imp (T : TyTree) (R : TyTree) : TyTree
+| tyTree_FATele {m : MTele} (T : MTele_Ty m) (F : forall t : MTele_val T, TyTree) : TyTree
+| tyTree_FA (T : Type) (F : T -> TyTree) : TyTree
+| tyTree_FAType (F : Type -> TyTree) : TyTree
+| tyTree_base (T : Type) : TyTree
 .
 
 Fixpoint tree_ty (X : TyTree) : Type :=
   match X as X' with
-  | tyTree_M _ T => M T
-  | tyTree_imp _ T R => tree_ty T -> tree_ty R
-  | @tyTree_FATele _ m T F => forall T, tree_ty (F T)
-  | tyTree_FA _ T F => forall t : T, tree_ty (F t)
-  | tyTree_FAType _ F => forall T : Type, F T 
-  | tyTree_ow _ T => T
+  | tyTree_val T => MTele_val T
+  | tyTree_M T => M T
+  | tyTree_MFA T => MFA T
+  | tyTree_In s F => MTele_val (MTele_In s F)
+  | tyTree_imp T R => tree_ty T -> tree_ty R
+  | @tyTree_FATele m T F => forall T, tree_ty (F T)
+  | tyTree_FA T F => forall t : T, tree_ty (F t)
+  | tyTree_FAType F => forall T : Type, tree_ty (F T)
+  | tyTree_base T => T
   end.
 
 Definition ty_tree (X : Type) : M TyTree :=
-  (mfix2 rec (X : Type) (p : bool) : M TyTree :=
+  (mfix1 rec (X : Type) : M TyTree :=
     mmatch X as X return M TyTree with
+    (* | [? (m : MTele) (T : MTele_Ty m)] MTele_val T =>
+       ret (tyTree_val p T) (* fail *) *)
     | [? T : Type] (M T):Type =>
-      ret (tyTree_M p T)
+      ret (tyTree_M T)
+    (* | [? (m : MTele) (T : MTele_Ty m)] (MFA T):Type =>
+      ret (tyTree_MFA T) (* fail *) *)
     | [? T R : Type] T -> R =>
-      T <- rec T (negb p);
-      R <- rec R p;
-      ret (tyTree_imp p T R) 
-    | [? (m : MTele) (T : MTele_Ty m) (F : forall x : MTele_val T, Type)] forall T , F T =>
+      T <- rec T ;
+      R <- rec R;
+      ret (tyTree_imp T R)
+    (* | [? (m : MTele) (T : MTele_Ty m) (F : forall x : MTele_val T, Type)] forall T , F T =>
       \nu t : _,
         F <- rec (F t) p;
         F <- abs_fun t F;
-        ret (tyTree_FATele p T F)  
+        ret (tyTree_FATele p T F) (* fail *) *)
+    | [? F : Type -> Type] forall T : Type, F T =>
+      \nu T : Type,
+        F <- rec (F T);
+        F <- abs_fun T F;
+        ret (tyTree_FAType F)
     | [? T (F : forall t : T, Type)] forall t : T, F t =>
       \nu t : T,
-        F <- rec (F t) p;
-        F <- abs_fun t F; (* Maybe abs_prod_type ? *)
-        ret (tyTree_FA p T F)
-    | [? F : Type -> Type] forall T : Type, F T =>
-      ret (tyTree_FAType p F)
-    | _ => ret (tyTree_ow p X) 
-    end) X true.
+        F <- rec (F t);
+        F <- abs_fun t F;
+        ret (tyTree_FA T F)
+    | _ => ret (tyTree_base X)
+    end) X.
 
 Definition ty_tree' {X : Type} (x : X) := ty_tree X.
 
-Goal M TyTree.
-mrun (ty_tree' (@bind)).
-w
+(* pol means polarity at that point of the tree *)
+(* We don't want the M at the return type *)
+Fixpoint checker (pol : bool) (X : TyTree) : Prop :=
+  match X as X' with
+  (* direct telescope cases *)
+  | tyTree_val T =>
+    match negb pol with
+    | true => True
+    | false => False
+    end
+  | tyTree_MFA T =>
+    match negb pol with
+    | true => True
+    | false => False
+    end
+  | tyTree_In s F =>
+    match negb pol with
+    | true => True
+    | false => False
+    end
+  | @tyTree_FATele m T F => forall t : MTele_val T, (checker pol (F t))
+  (* non-telescope cases *)
+  | tyTree_M T => True
+  | tyTree_base T => True
+  (* indirect cases *)
+  | tyTree_imp T R => match checker (negb pol) T with
+                     | True => checker pol R
+                     end
+  | tyTree_FA T F => forall t : T, checker pol (F t)
+  | tyTree_FAType F => forall T : Type, checker pol (F T)
+  end.
+
+
+Goal TyTree.
+mrun (ty_tree' (@ret)).
+Show Proof.
+
+Goal TyTree.
+mrun (ty_tree'(@bind)).
+Show Proof.
+
+Goal TyTree.
+mrun (ty_tree (forall (m : MTele) (A B : MTele_Ty m), MFA A -> (MTele_val A -> MFA B) -> MFA B)).
+Show Proof.
+
+Notation "'[withP' now_ty , now_val '=>' t ]" :=
+  (MTele_In (SProp) (fun now_ty now_val => t))
+  (at level 0, format "[withP now_ty , now_val => t ]").
+
+Eval compute in (tree_ty (tyTree_base nat)).
+Eval compute in (tree_ty (tyTree_FAType (fun T : Type => tyTree_imp (tyTree_base T) (tyTree_M T)))).
+
+Eval compute in (checker true (tyTree_FAType (fun T : Type => tyTree_imp (tyTree_base T) (tyTree_M T)))).
+Eval compute in (checker true (tyTree_FA MTele
+   (fun t0 : MTele =>
+    tyTree_FA (MTele_Ty t0)
+      (fun t1 : MTele_Ty t0 =>
+       tyTree_FA (MTele_Ty t0)
+         (fun t2 : MTele_Ty t0 =>
+          tyTree_imp (tyTree_MFA t1)
+            (tyTree_imp
+               (tyTree_imp (tyTree_val t1)
+                  (tyTree_MFA t2)) (tyTree_MFA t2))))))).
